SStructTT/SStruct/Static/Step.lean
@@ -78,9 +78,9 @@ inductive Step : Tm Srt -> Tm Srt -> Prop where
   | ite_N2 A m n1 {n2 n2'} :
     Step n2 n2' ->
     Step (.ite A m n1 n2) (.ite A m n1 n2')
-  | ite_true A n1 n2 :
+  | ite_tt A n1 n2 :
     Step (.ite A .tt n1 n2) n1
-  | ite_false A n1 n2 :
+  | ite_ff A n1 n2 :
     Step (.ite A .ff n1 n2) n2
   | idn_A {A A'} m n :
     Step A A' ->
